Day 25: Christmas part1

problems/25/Problem25.dfy
@@ -1,6 +1,129 @@
+include "../../parser/split.dfy"
 module Problem25 {
+    import opened Split
+    import opened Std.Collections.Seq
+    type Lock = seq<nat>
+    type Key = seq<nat>
+
+    predicate IsLock(x: seq<string>) 
+        requires |x| > 0
+    {
+        forall i :: 0 <= i < |x[0]| ==> x[0][i] == '#'
+    }
+
+    method MeasureHeights(x: seq<string>) returns (heights: seq<nat>)
+        requires |x| >= 7
+        requires forall i :: 0 <= i < 7 ==> |x[i]| == 5
+        ensures |heights| == 5
+        ensures forall i :: 0 <= i < 5 ==> 1 <= heights[i] < 7
+    {
+        heights := [];
+        for i := 0 to 5 
+            invariant |heights| == i
+            invariant forall j :: 0 <= j < i ==> 0 < heights[j] < 7
+        {
+            var height := 0;
+            for j := 0 to 7 {
+                if x[j][i] == '#' {
+                    height := height + 1;
+                }
+            }
+            expect 0 < height < 7;
+            heights := heights + [height];
+        }
+    }
+
+    method parseInput(input: string) returns (locks: seq<Lock>, keys: seq<Key>) 
+        ensures forall i :: 0 <= i < |locks| ==> |locks[i]| == 5
+        ensures forall i :: 0 <= i < |keys| ==> |keys[i]| == 5
+        ensures forall i :: 0 <= i < |locks| ==> forall j :: 0 <= j < 5 ==> 1 <= locks[i][j] < 7
+        ensures forall i :: 0 <= i < |keys| ==> forall j :: 0 <= j < 5 ==> 1 <= keys[i][j] < 7
+    {
+        locks := [];
+        keys := [];
+        var data := splitOnDoubleBreak(input);
+        for i := 0 to |data| 
+            invariant forall lock :: 0 <= lock < |locks| ==> |locks[lock]| == 5
+            invariant forall key :: 0 <= key < |keys| ==> |keys[key]| == 5
+            invariant forall lock :: 0 <= lock < |locks| ==> forall j :: 0 <= j < 5 ==> 1 <= locks[lock][j] < 7
+            invariant forall key :: 0 <= key < |keys| ==> forall j :: 0 <= j < 5 ==> 1 <= keys[key][j] < 7
+        {
+            if data[i] != "" {
+                var lines := splitOnBreak(data[i]);
+                // print lines, "\n";
+                expect |lines| >= 7;
+                expect forall j :: 0 <= j < 7 ==> |lines[j]| == 5;
+                if IsLock(lines) {
+                    var heights := MeasureHeights(lines);
+                    locks := locks + [heights];
+                } else {
+                    var heights := MeasureHeights(lines);
+                    keys := keys + [heights];
+                }
+            }
+        }
+    }
+
     method problem25_1(input: string) returns (x: int) {
-        return 3;
+        var locks, keys := parseInput(input);
+        print locks, "\n";
+        print keys, "\n";
+        var groups: map<nat, map<nat, set<Key>>> := map[];
+        for j := 0 to 5 
+            invariant forall k :: 0 <= k < j ==> k in groups
+            invariant forall k :: 0 <= k < j ==> forall l :: 0 <= l < 7 ==> l in groups[k]
+        {
+            groups := groups[j := map[]];
+            for k := 0 to 7 
+                invariant forall i :: 0 <= i < j ==> i in groups
+                invariant forall k :: 0 <= k < j ==> forall l :: 0 <= l < 7 ==> l in groups[k]
+                invariant j in groups
+                invariant forall i :: 0 <= i < k ==> i in groups[j]
+            {
+                groups := groups[j := groups[j] + groups[j][k := {}]];
+            }
+        }
+        assert forall i :: 0 <= i < 5 ==> i in groups;
+        assert forall i :: 0 <= i < 5 ==> forall j :: 0 <= j <= 6 ==> j in groups[i];
+        for i := 0 to |keys| 
+            invariant forall k :: 0 <= k < 5 ==> k in groups
+            invariant forall i :: 0 <= i < 5 ==> forall j :: 0 <= j <= 6 ==> j in groups[i]
+        {
+            var key := keys[i];
+            for j := 0 to 5 
+                invariant forall k :: 0 <= k < 5 ==> k in groups
+                invariant forall i :: 0 <= i < 5 ==> forall j :: 0 <= j <= 6 ==> j in groups[i]
+                // invariant 0 <= j <= 5 && j in groups
+                // invariant forall z :: 0 <= z < j ==> key[j] < 7
+            {
+                for k := key[j] to 7
+                    invariant forall k :: 0 <= k < 5 ==> k in groups
+                    invariant forall i :: 0 <= i < 5 ==> forall j :: 0 <= j <= 6 ==> j in groups[i]
+                    invariant key[j]+1 <= 7
+                {
+
+                    groups := groups[j := groups[j][k := groups[j][k] + {key}]];
+                }
+            }
+        }
+        // print groups[0], "\n\n";
+        // print groups[1], "\n\n";
+        // print groups[2], "\n\n";
+        // print groups[3], "\n\n";
+        // print groups[4], "\n\n";
+        x := 0;
+        for i := 0 to |locks| 
+        {
+            // print "Lock ", i," ", locks[i], "\n";
+            var possibleKeys: set<Key> := groups[0][7-locks[i][0]];
+            // print possibleKeys, "\n";
+            for j := 1 to 5 
+            {
+                // print groups[j][6-locks[i][j]], "\n";
+                possibleKeys := possibleKeys * groups[j][7-locks[i][j]];
+            }
+            x := x + |possibleKeys|;
+        }
     }
 
     method problem25_2(input: string) returns (x: int) {
